Upd

Spec.Claim.fst
@@ -1,7 +1,38 @@
 module Spec.Claim
 
+open FStar.Seq
 
+let bytes =  seq FStar.UInt8.t
+
+type keyEnt = 
+|InitKeyEnt : source: string -> key: bytes -> keyEnt
+
+type indentifier = 
+|InitIndent : source: string -> identifier : option string -> indentifier
+
+assume val hash: list 'a -> bytes
+
+type metadata = 
+|InitMetadata: screen_name: option string ->
+				real_name: option string -> 
+				identifiers: list indentifier -> 
+				keys: list keyEnt -> 
+				hashMetadata: bytes ->
+				metadata
+
+
+
+assume val sign : input: bytes -> bytes
+assume val verify : signature: bytes -> data: bytes -> Tot bool
+
+assume val toBytes: input : 'a -> bytes
+assume val concat: bytes-> bytes -> bytes
+
+(* Authenticity of information *)
 type claim = 
-	|InitClaim: test: list int -> claim
+	|InitClaim: test: list int -> signature : bytes{verify signature (toBytes test) } -> claim (* test purposes*)
+	|KeyBindingClaim: meta: metadata -> key: bytes -> signature : bytes {verify signature (concat (toBytes meta) (toBytes key))}  -> claim
+	|ClaimChainState: id: bytes -> state: bytes-> signature : bytes{verify signature (concat id state)} -> claim
+	|Revocation: id: bytes -> signature : bytes{verify signature id}-> claim
 
 
